\documentclass{ximera}

\input{../preamble.tex}


\title[Problem 1]{Problem 1}

\begin{document}
\begin{abstract} \end{abstract}
\maketitle


% Extracted from approximatingTheAreaUnderACurve.tex, problem #1
\begin{problem} Evaluate the sum.
\begin{enumerate}
	\item  $\sum_{k=1}^{n}5$
		\begin{explanation}
		  $\sum_{k=1}^{n}5=n\cdot5$
		\end{explanation}	
\item  $\sum_{k=1}^{10}5$
		\begin{explanation}
			Using the previous result for $n=10$, we get
 			$\sum_{k=1}^{10}5=10\cdot5=50$\\
  			or\\

   			$\sum_{k=1}^{10}5=5+5+5+5+5+5+5+5+5+5=50$
		\end{explanation}	
\item  $\sum_{k=1}^{n}8k$
		\begin{explanation}
  			$\sum_{k=1}^{n}8k=8\sum_{k=1}^{n}k=8\frac{n(n+1)}{2}=4n(n+1)$
		\end{explanation}	

\vspace*{\stretch{1}}
	\item  $\sum_{k=1}^{4}8k$
		\begin{explanation}
			Using the previous result for $n=4$, we get
			  $\sum_{k=1}^{4}8k=4(4)(4+1)=80$\\
			  or\\
			  $\sum_{k=1}^{4}8k=8(1)+8(2)+8(3)+8(4)=8+16+24+32=80$
		\end{explanation}	
\item  $\sum_{k=1}^{n}(6k^2-8k-5)$	
		\begin{explanation}
			$\sum_{k=1}^{n}(6k^2-8k-5)=\sum_{k=1}^{n}6k^2+\sum_{k=1}^{n}(-8k)+\sum_{k=1}^{n}(-5)=$\\
			$=6\sum_{k=1}^{n}k^2-8\sum_{k=1}^{n}k-\sum_{k=1}^{n}5=$ \\
			Now we use the formulas.\\[1em]
			$=6\frac{n(n+1)(2n+1)}{6}-8\frac{n(n+1)}{2}-\sum_{k=1}^{n}5=n(n+1)(2n+1)-4n(n+1)-5n$=\\[1em]
			$=2n^3-n^2-8n$
		\end{explanation}	
\item  $\sum_{k=0}^{2} \cos\left( \dfrac{\pi}{2}k\right)$
		\begin{explanation}
		\begin{align*}
			\sum_{k=0}^{2} \cos\left( \dfrac{\pi}{2}k\right) &= \cos\left( \dfrac{\pi}{2}(0)\right) + \cos\left( \dfrac{\pi}{2}(1)\right) + \cos\left( \dfrac{\pi}{2}(2)\right)\\
			&= \cos\left( 0\right) + \cos\left( \dfrac{\pi}{2}\right) + \cos\left( \pi\right) \\
			&= 1 + 0 + -1 = 0.
		\end{align*}
		\end{explanation}
\end{enumerate}
\end{problem}



\end{document}
