\documentclass{ximera}

\input{../preamble.tex}


\title[Problem 9]{Problem 9}

\begin{document}
\begin{abstract} \end{abstract}
\maketitle


% Extracted from meanValueTheorem.tex, problem #9
\begin{problem}
  Let $f(x) = (x-3)^{-2}$.
  Show that there is no value $c$ in $(1,4)$ such that $f(4) - f(1) = f^{\prime}(c) (4-1)$.
  Why does this not contradict the Mean Value Theorem?
\begin{explanation}
    First notice that 
    $$f(4)-f(1) = 1^{-2} - (-2)^{-2} = 1-\frac{1}{4} = \frac{3}{4}$$
    and so we are looking for a value $c$ such that 
    $$3 f^\prime (c) = \frac{3}{4} \quad \Longrightarrow \quad f^\prime (c) = \frac{1}{4} $$
    Then since $f'(x) = \frac{-2}{(x-3)^3}$, we can compute:
    $$ f'(c) = \frac{-2}{(c-3)^3} := \frac{1}{4}$$
    $$ (c-3)^3 = - 8 $$
    $$ c = 3 - 2 = 1 $$
    But $1$ is not in the interval $(1,4)$.  This does not contradict the Mean Value Theorem since $f$ is not continuous at $x=3$.

    \begin{image}
      \includegraphics[scale=.65]{ifigure5.png}
    \end{image}
  \end{explanation}
\end{problem}



\end{document}
