% Extracted from rulesOfDifferentiation.tex, problem #4
\begin{problem}

  Use the given graphs of $f$ and $g$ and their accompanying derivatives to answer the following questions.
  \begin{image}
    \hspace*{-7em}
     \includegraphics[scale = 0.3]{graphSquaringFunction.png}
     \hspace{2em}
     \includegraphics[scale = 0.3]{graphSquaringFunctionDeriv.png}
   \end{image}
   \begin{image}
     \includegraphics[scale = 0.23]{graphIdentityFunction.png}
   \end{image}

   \begin{enumerate}
     \item
	Write an equation for the tangent line to $f$ at $x=2$.
\WkstHop
	\begin{freeResponse}
	$f(2)=4$,\quad $f'(2)=4$, \quad $y-4=4(x-2)$, \quad $y=4x-4$
	\end{freeResponse}

	\item Draw the graph of $g'$
	\WkstHop
		\begin{freeResponse}
	   \begin{image}
     \includegraphics[scale = 0.23]{graphIdentityFunctionDeriv.png}
   \end{image}	
		\end{freeResponse}
       \item Compute the value of the $(5f+3g)'(2)$.
\WkstHop
       \begin{freeResponse}
         \begin{align*}
           (5f+3g)'(2) &= 5\cdot f'(2) + 3 \cdot g'(2)\\
                       &= 5 \cdot 4 + 3 \cdot 1 \\
                       &= 20 + 3 = 23.
         \end{align*}
       \end{freeResponse}

	\item Find the equation of the tangent line to the graph of $(5f+3g)$ at the point where $x=2$.
\WkstHop
	\begin{freeResponse}
         \begin{align*}
           (5f+3g)(2) &= 5\cdot f(2) + 3 \cdot g(2)\\
                       &= 5 \cdot 4 + 3 \cdot 2 \\
                       &= 20 + 6 = 26\\\\
	y-26 &=23(x-2)\\
	y&=23x-20
         \end{align*}
	\end{freeResponse}

	\item Use the given graph of $f'$ and $g'$ to find the following:
	\begin{enumerate}
		\item A formula for $f'$
\WkstHop
			\begin{freeResponse}
				$f'(x)=2x$.  The graph shows a linear function through the point $(0,0)$ and $(1,2)$.
			\end{freeResponse}
	
		\item A formula for $g'$
\WkstHop
			\begin{freeResponse}
				$g'(x)=1$.  The graph shows a linear function with slope $0$ and through the point $(0,1)$.
			\end{freeResponse}
	\end{enumerate}

	\item Find the expression for $(5f+3g)'(x)$.
\WkstHop	
	\begin{freeResponse}
         \begin{align*}
           (5f+3g)'(x) &= 5\cdot f'(x) + 3 \cdot g'(x)\\
                       &= 5 \cdot 2x + 3 \cdot 1 \\
                       &= 10x+3
         \end{align*}
	\end{freeResponse}

  

   \end{enumerate}

\end{problem}
