\documentclass{ximera}

\input{../../preamble.tex}


\title[Problem 5]{Problem 5}

\begin{document}
\begin{abstract} \end{abstract}
\maketitle


% Extracted from productRuleAndQuotientRule.tex, problem #5
\begin{problem}
Differentiate the following functions:

	\begin{enumerate}
	
	%part a
	\item  Given $f(x) = (x^2 + 4x - 7) e^{-x}$, show $f'(x)= (11-x^2 -2x) e^{-x}$.
\begin{explanation}
			\begin{align*}
			f'(x) &= \ddx \Bigl(\frac{x^2 + 4x - 7}{e^{x}}\Bigr)  \\
			&= \frac{(2x+4)e^{x}-(x^2 + 4x - 7)e^{x}}{e^{2x}} \\
			&= \frac{e^{x}(2x + 4-x^2 - 4x + 7)}{e^{2x}} \\ 
			&=  \frac{11-x^2 - 2x }{e^{x}} \\ 
			&=(11-x^2 -2x) e^{-x}
			\end{align*}
			\end{explanation}
			
			
			
	%part b
	\item  Given $g(x) = \frac{x^2 + 4x - 7}{e^{-x}}$, show $g'(x)=\frac{x^2 + 6x - 3}{e^{-x}}$
\begin{explanation}
			\begin{align*}
			g'(x) &=  \ddx \Bigl(\frac{x^2 + 4x - 7}{e^{-x}}\Bigr)  \\
			&= \ddx \Bigl((x^2 + 4x - 7)e^{x} \Bigr) \\
			&= \ddx(x^2 + 4x - 7)e^{x} +(x^2 + 4x - 7)\ddx e^{x}\\
			&=(2x+4)e^{x}+(x^2 + 4x - 7)e^{x}\\
			&=e^{x}(2x+4+x^2 + 4x - 7)\\
			&=e^{x}(x^2 + 6x - 3)\\
			&=\frac{x^2 + 6x - 3}{e^{-x}}\\
			\end{align*}
			\end{explanation}
			
	\end{enumerate}		
\end{problem}



\end{document}
