% Extracted from limitLaws.tex, problem #2
\begin{problem}
Find the limit and justify your answer.
\begin{enumerate}
	\item $\displaystyle \lim_{x \to 0}|x|$
\WkstHop	
	\begin{freeResponse}
		
Remember
\hspace{0.2in}$|x| =   \left\{ \begin{array}{lr}
	-x 	&	\text{if } x < 0	\\
	x	&	\text{if } x \ge 0	\end{array} \right.  $\\	
We first compute the one-sided limit: 
	$ \lim_{x \to 0^{+}} |x|=  \lim_{x \to 0^{+}} x= 0$.\\	
Next, we compute the other one-sided limit:\\
	$ \lim_{x \to 0^{-}} |x|=  \lim_{x \to 0^{-}} (-x)= \Big(\lim_{x \to 0^{-}} (-1)\Bigr)\Bigl(\lim_{x \to 0^{-}} x\Bigr)=(-1)(0)=0$.\\[1em]	
Therefore	
	$ \lim_{x \to 0^{-}} |x|=0=\lim_{x \to 0^{+}} |x|$.
Hence,
$ \lim_{x \to 0} |x| =0 $.
\end{freeResponse}


\item $\displaystyle \lim_{x \to 2} \ln{\Bigl(\sin{(x-2)}+e^{x}\sin\left({\dfrac{\pi x}{4}}\right)\Bigr)}$

\WkstHop
\begin{freeResponse}
	\begin{align*}
		\lim_{x \to 2} \ln\left(\sin(x-2)+e^{x}\sin\left(\dfrac{\pi x}{4}\right) \right) 
			&= \ln\left( \lim_{x \to 2} \left( \sin(x-2)+e^{x}\sin\left(\dfrac{\pi x}{4}\right) \right) \right) \\
			&= \ln\left( \lim_{x \to 2} \sin(x-2)+\lim_{x \to 2} \left(e^{x}\sin\left(\dfrac{\pi x}{4}\right) \right) \right) \\
			&= \ln\left( \sin\left(\lim_{x \to 2}(x-2)\right)+\left(\lim_{x \to 2} e^{x}\right)\left(\lim_{x \to 2}\sin\left(\dfrac{\pi x}{4}\right) \right) \right) \\
			&= \ln\left( \sin(0)+\left(\lim_{x \to 2} e^{x}\right)\sin\left(\lim_{x \to 2}\dfrac{\pi x}{4}\right) \right) \\
			&= \ln\left( 0+e^2 \sin\left(\dfrac{2\pi}{4}\right) \right) \\
			&= \ln\left( e^2 \sin\left(\dfrac{\pi}{2}\right) \right) = \ln\left( e^2 (1) \right) \\
			&= \ln\left( e^2 \right) = 2
	\end{align*}
\end{freeResponse}

\item $\displaystyle \lim_{x \to 1} \dfrac{3+2\cos\left(\frac{\pi x}{3}\right)}{4x-2x^{3}}$
\WkstHop
\begin{freeResponse}
	\begin{align*}
		\lim_{x\to 1} \frac{3+2\cos\left(\frac{\pi x}{3}\right)}{4x-2x^3} 
			&= \frac{\lim_{x\to 1}\left(3+2\cos\left(\frac{\pi x}{3}\right)\right)}{\lim_{x\to 1}\left(4x-2x^3\right)}\\
			&= \frac{\lim_{x\to 1}(3) +\lim_{x\to 1}\left(2\cos\left(\frac{\pi x}{3}\right)\right)}{4(1)-2(1)^3}\\	
			&= \frac{3 +\left(\lim_{x\to 1}2\right)\left(\lim_{x\to 1}\cos\left(\frac{\pi x}{3}\right)\right)}{4-2(1)}\\	
			&= \frac{3 +2\cos\left(\lim_{x\to 1}\frac{\pi x}{3}\right)}{4-2}\\	
			&= \frac{3 +2\cos\left(\frac{\pi}{3}\right)}{2} = \frac{3 +2\left(\frac{1}{2}\right)}{2}\\	
			&= \frac{3+1}{2} = 2.
	\end{align*}

\end{freeResponse}
\end{enumerate}
\end{problem}
