\documentclass{ximera}

\input{../preamble.tex}


\title[Problem 1]{Problem 1}

\begin{document}
\begin{abstract} \end{abstract}
\maketitle


% Extracted from chainRule.tex, problem #1
\begin{problem}
For the following problems, the derivative is given.  Determine which function was the original function.
	\begin{enumerate}
	
		\item  The derivative is $f'(x) = \cos (x) e^{\sin (x)}$.  Which is the original function?
		
			\begin{enumerate}
			\item  $f(x) = (\sin(x))(e^x)$
			\item  $f(x) = \sin (e^x)$
			\item  $f(x) = e^{\sin(x)}$
			\item  $f(x) = e^{x \sin(x)}$

				\begin{explanation}
				Since
				$$ \ddx \left( e^{\sin(x)} \right) = e^{\sin(x)} \cdot \cos(x) = \cos(x) e^{\sin(x)} $$
				the correct answer is (iii).  
				\end{explanation}
				
			\end{enumerate}
			
			\item  The derivative is $g'(x) = 4 \left( \tan (x^4 - 5x) \right)^3 \sec^2(x^4-5x)(4x^3-5)$.  Which is the original function?
		
			\begin{enumerate}
			
			\item  $g(x) = \left( \tan(x) - 5x \right)^4$
			\item  $g(x) = \tan^4(x) - 5x^4$
			\item  $g(x) = \tan(x^4 - 5x)$
			\item  $g(x) = \tan^4(x^4-5x)$
			
				\begin{explanation}
				Since 
				$$\ddx \left( \tan^4(x^4-5x) \right) = 4 \tan^3(x^4-5x) \sec^2(x^4-5x) (4x^3-5)$$ 
				the correct answer is (iv).  Notice that $\tan^3(x^4-5x) = \left( \tan(x^4-5x) \right)^3$ are (slightly) different notations for the exact same expression.
				\end{explanation}
				
			\end{enumerate}
\end{enumerate}
\end{problem}



\end{document}
