\documentclass{ximera}

\input{../preamble.tex}


\title[Problem 4]{Problem 4}

\begin{document}
\begin{abstract} \end{abstract}
\maketitle


% Extracted from productRuleAndQuotientRule.tex, problem #4
\begin{problem}
  Use the given information to find the equation of the tangent line.
  \begin{enumerate}
    \item
      Given $g(x) = x^3 f(x)$, $f(2) = 4$, and $f'(2) = 7$, find the equation of the tangent line to the graph of $g$ at $x = 2$.
\begin{explanation}
        Slope of tangent line to the graph of $g$ at the point where $x = 2$:
        \begin{align*}
          g'(x) &= 3x^2 f(x) + x^3 f'(x)\\
          &\implies g'(2) = 12(4) + 8(7) = 48 + 56 = 104.
        \end{align*}

        Point on tangent line where $x=2$: $(2, g(2)) = (2, 8f(2)) = (2, 32)$.

        Equation of tangent line:
        \begin{align*}
          y-32 &= 104(x-2)\\
          &\implies y = 104x - 176.
        \end{align*}
      \end{explanation}


    \item
      Given $h(z) = \frac{z s(z)}{z-3}$, $s(2) = 4$, and $s'(2) = 7$, find the equation of the tangent line to the graph of $h$ at $z = 2$.
\begin{explanation}
        Slope of tangent line to the graph of $h$ at the point where $z = 2$:
        \begin{align*}
          h'(z) &= \frac{ (z-3)(z s(z))' - z s(z)(z-3)'}{(z-3)^2}  \\
		&= \frac{(z-3)(s(z) + z s'(z)) - z s(z)(1)}{(z-3)^2} \\
                &\implies h'(2) = \frac{(2-3)(s(2) + 2 s'(2)) - 2s(2)}{(2-3)^2} = -26.
        \end{align*}

        Point on tangent line where $z=2$: $(2, h(2)) = (2, \frac{2s(2)}{2-3}) = (2, -8)$.

        Equation of tangent line to the graph of $h$ at the point where $z=2$:
        \begin{align*}
          y-(-8) &= -26(z-2) \\
          &\implies y = -26z + 44.
        \end{align*}
      \end{explanation}


    \item
      Given
      \begin{center}
        \begin{tabular}{cccccc}
       \toprule
          $x$ & 1 & 2 & 3 & 4 & 5\\
     \midrule
          $f(x)$ & 5 & 3 & 0 &$-4$ & 3\\
          $f'(x)$ & $-3$ & $-5$ & $-2$ & 6& $-4$\\
          $g(x)$ & 6 &9&$-8$&13&15\\
          $g'(x)$ & 8 & 5 & $-10$ &7& 6\\
  	\bottomrule
        \end{tabular}
      \end{center}
      find the equation of the tangent line of 
      \[
        \frac{f(x)}{e^xg(x)}
      \]
      at $x = 2$.
\begin{explanation}
        Slope of tangent line to the graph of $ \frac{f(x)}{e^xg(x)} $ at the point where $x=2$:
        \begin{align*}
          \left( \frac{f(x)}{e^x g(x)} \right)'
          &= \frac{e^x g(x) f'(x) - f(x)(e^x g(x) + e^x g'(x))}{(e^x g(x))^2}.  \\
          &\implies \frac{d}{dx}\left(\frac{f(x)}{e^x g(x)}\right) \bigg|_{x=2}
          = \frac{e^2 g(2) f'(2) - f(2)(e^2 g(2) + e^2 g'(2))}{(e^2 g(2))^2}  \\
		&= \frac{e^2 (9)(-5) - (3)(9e^2 + 5e^2)}{(9e^2)^2}  \\
		&= \frac{-45e^2 -42e^2}{81e^4}  \\
		&= \frac{-87e^2}{81e^4}\\
                  &= \frac{-87}{81e^2}
        \end{align*}

        Point on tangent line where $x=2$: $(2, f(2)/(e^2g(2))) = (2, 3/(9e^2)) = (2, 1/(3e^2))$.

        Equation of tangent line where $x=2$:
        \begin{align*}
          y - \frac{1}{3e^2} &= \frac{-87}{81e^2}(x - 2)\\
                             &\implies y = \frac{-87}{81e^2}x  + \frac{67}{27e^2}.
        \end{align*}
      \end{explanation}
   \end{enumerate}
\end{problem}



\end{document}
