\documentclass{ximera}

\input{../../preamble.tex}


\title[Problem 1]{Problem 1}

\begin{document}
\begin{abstract} \end{abstract}
\maketitle


% Extracted from substitution.tex, problem #1
\begin{problem}
	Compute the following indefinite integrals.
	\begin{enumerate}
		\item $\displaystyle \int 2t \sin(t^2) \, \d t$.
			\begin{explanation}
        		Let $w=t^2$. Then $\d w = 2t \, \d t$ so
        		\begin{align*}
        			\int 2t \sin(t^2) \, \d t &= \int \sin(2) \, \d w\\
        				&= -\cos(w) + C\\
        				&= -\cos(t^2) + C.
        		\end{align*}
        	\end{explanation}
	
		\item $\displaystyle \int \cos(x) \sqrt{\sin(x)} \, \d x$.
	\begin{explanation}
		Set $v = \sin(x)$. Then $dv = \cos(x) \, dx$, so
		\begin{align*}
			\int \cos(x) \sqrt{\sin(x)} \, \d x &= \int \sqrt{v} \, dv\\
				&= \dfrac{2}{3} v^{3/2} + C\\
				&= \dfrac{2}{3} (\sin(x))^{3/2} + C
		\end{align*}
	\end{explanation}
		
	\item $\displaystyle \int \left( 3t^2-4+\dfrac{1}{t} \right) e^{t^3-4t+\ln(t)-9}\, \d t$.
	\begin{explanation}
		This problem looks a lot more difficult than it really is. Let $u = t^3-4t+\ln(t)-9$. Then $\d u = \left( 3t^2- 4+\dfrac{1}{t} \right) \, \d t$, 
		which is exactly the factor in front of the exponential.
		\begin{align*}
			\int \left( 3t^2-4+\dfrac{1}{t} \right) e^{t^3-4t+\ln(t)-9}\, \d t &= \int e^u \, \d u\\
				&= e^u + C\\
				&= e^{t^3-4t+\ln(t)-9}+C.
		\end{align*}
	\end{explanation}

	\end{enumerate}
	
\end{problem}



\end{document}
