\documentclass{ximera}

\input{../../preamble.tex}


\title[Problem 3]{Problem 3}

\begin{document}
\begin{abstract} \end{abstract}
\maketitle


% Extracted from implicitDifferentiation.tex, problem #3
\begin{problem}  A part of the curve with equation $\cos(\pi x y) + x + y = 1$ is sketched below.

  \begin{image}
    \includegraphics[scale = 0.3]{figure4.png}
  \end{image}
  \begin{enumerate}
    \item
      Use the implicit differentiation to find the derivative $dy/dx$.
\begin{explanation}
        Implicitly differentiate equation:
        \begin{align*}
          \ddx( \cos(\pi x y) + x + y) = \ddx(1) &\implies -\sin(\pi x y)\cdot(\pi y + \pi x \dd[y]{x}) + 1 + \dd[y]{x} = 0 
        \end{align*}

        Solve for $\dd[y]{x}$:
        \begin{align*}
          -\sin(\pi x y)\cdot(\pi y + \pi x \dd[y]{x}) + 1 + \dd[y]{x} = 0 &\implies -\pi y \sin(\pi x y) - \pi x \dd[y]{x} \sin(\pi x y) + 1 + \dd[y]{x} = 0 \\
          &\implies  \bigl(1 - \pi x \sin(\pi x y)\bigr)\dd[y]{x} = \pi y \sin(\pi x y) - 1 \\
          &\implies \dd[y]{x} = \frac{\pi y \sin(\pi x y) - 1}{1 - \pi x \sin(\pi x y)} \hspace{2em} \mbox{if $1 - \pi x \sin(\pi x y) \ne 0$}\\
        \end{align*}
      \end{explanation}

    \item
      Consider the point $(1, 1)$.
      Show (algebraically) that this point lies on the curve.
\begin{explanation}
        $(1, 1)$ lies on this curve:
        \begin{align*}
          \cos(\pi \cdot 1 \cdot 1) + 1 + 1 &= \cos(\pi) + 2\\
          &= -1 + 2 = 1
        \end{align*}
      \end{explanation}

    \item
      Find the equation of the line tangent to the curve at $(1,1)$.
      Draw this line in the figure above.
\begin{explanation}
        Slope of tangent line:
        \begin{align*}
          \eval{\dd[y]{x}}_{(1,1)} &= \frac{\pi \cdot (1) \cdot\sin(\pi (1) \cdot 1) - 1}{1 - \pi \cdot (1) \cdot \sin(\pi (1) \cdot (1))} \\
          &= \frac{\pi\sin(\pi) - 1}{1 - \pi \sin(\pi)}\\
          &= \frac{-1}{1} = -1
        \end{align*}

        Equation of tangent line:
        \begin{align*}
          y - 1 = -1(x - 1) &\implies y = -x + 2
        \end{align*}

        Graph of tangent line:
        \begin{image}
          \includegraphics[scale = 0.5]{figure5.png}
        \end{image}
      \end{explanation}

  \end{enumerate}
\end{problem}



\end{document}
