\documentclass{ximera}

\input{../preamble.tex}


\title[Problem 3]{Problem 3}

\begin{document}
\begin{abstract} \end{abstract}
\maketitle


% Extracted from moreThanOneRate.tex, problem #3
\begin{problem}
A part of a circle centered at the origin with radius $r=7$ cm is given in the figure (A) below.  A right triangle is formed in the first quadrant (see Figure (A)).  One of its sides lies on the $x$-axis.  Its hypotenuse runs from the origin to a point on the circle.  The hypotenuse makes an angle $\theta$ with the $x$-axis.  Assume that the angle $\theta$ changes at the rate $\frac{d\theta}{dt}=0.2$\ radians per second.

	\begin{image}
		 
		\includegraphics[scale=.5]{Figure10.png}
	\end{image}
	
\begin{enumerate}
	\item Label Figure A.
		\begin{explanation} \hfil

		\begin{image}
		 
			\includegraphics[scale=.5]{Figure11.png}
		\end{image}
		
		\end{explanation}
		
	\item In Figure B, draw the the triangle twice; once when $\theta$ is small and once more, when $\theta$ is close to $\frac{\pi}{2}$.

		\begin{image}
		 
			\includegraphics[scale=.4]{Figure12.png}
		\end{image}
	
		\begin{explanation} \hfil
	
			\begin{image}
				 
				\includegraphics[scale=.5]{Figure13.png}
			\end{image}
	
		\end{explanation}
\item Find the rate of change of the height of the triangle when $\theta=\frac{\pi}{3}$
\begin{explanation}
		$y=7\sin{\theta}$
		\begin{align*}
		\frac{dy}{dt}&=\frac{dy}{d\theta}\cdot \frac{d\theta}{dt}\\
		\frac{dy}{dt}&=7\cos{\theta} \cdot \frac{d\theta}{dt}\\
		\eval{\frac{dy}{dt}}_{\theta=\frac{\pi}{3}}&=7(1/2)(0.2)\\
		&=0.7 \text{cm/sec}
		\end{align*}
				\end{explanation}
	\item Find the rate of change of the area of the triangle when $\theta=\frac{\pi}{3}$
\begin{explanation}
		First, we need to find $x$: $x=7 \cos{\theta}$.  From part c, we know $y=7\sin{\theta}$
		\begin{align*}
		A&=\frac{1}{2}xy\\
		A&=\frac{49}{2}\cos(\theta)\sin(\theta)\\
		\frac{dA}{dt}&=\frac{49}{2}(-\sin^2(\theta)+\cos^2(\theta)) \cdot \frac{d\theta}{dt}\\
		\eval{\frac{dA}{dt}}_{\theta=\frac{\pi}{3}}&=\frac{49}{2}\left(-\left(\frac{\sqrt{3}}{2}\right)^2+\left(\frac{1}{2}\right)^2 \right) \cdot 0.2\\\\
		&=\frac{49}{2}\cdot \frac{-1}{2} \cdot 0.2\\
		&=\frac{-4.9}{2} cm^2/sec
		\end{align*}
		\end{explanation}

\end{enumerate}
\end{problem}



\end{document}
