\documentclass{ximera}

\input{../../preamble.tex}


\title[Problem 3]{Problem 3}

\begin{document}
\begin{abstract} \end{abstract}
\maketitle


% Extracted from logarithmicDifferentiation.tex, problem #3
\begin{problem}
  True or False:
  \begin{enumerate}
    \item[(1)]
      If $f(x) = (x-2)^x$, then $f'(x) = x (x-2)^{x-1}$.
\begin{explanation}
        False.
        Any time that you have a function of $x$ raised to a function of $x$, in order to compute the derivative you need to use logarithmic differentiation (or something equivalent).

        Correct derivative of $f$:
        \begin{align*}
          f(x) &= (x-2)^x \implies f(x) = e^{x \ln(x-2)} \\
          &\implies f'(x) = e^{x \ln(x-2)} \cdot \left(1\cdot\ln(x-2) + x \cdot \frac{1}{x-2}\right) \\
          &\implies f'(x) = (x-2)^x \cdot \left(\ln(x-2) + \frac{x}{x-2}\right)
        \end{align*}
        \end{explanation}	
		
      \item[(2)]
        If $f(x) = (3x)^x$, then $f'(x) = (3x)^x \ln (3x)$.
\begin{explanation}
          False.  Same as part (1).

          Correct derivative of $f$:
          \begin{align*}
            f(x) &= (3x)^x \implies f(x) = e^{x \cdot \ln(3x)} \\
            &\implies f'(x)  = e^{x \cdot \ln(3x)} \left(1 \cdot \ln(3x) + x \cdot \frac{3}{3x} \right) \\
            &\implies f'(x)  = (3x)^x \left(\ln(3x) + 1 \right)
          \end{align*}
	\end{explanation}	
	\end{enumerate}
\end{problem}



\end{document}
